Define $s(x) = [x]$ and $f(x)=\frac{\log x}{x}$.
This yields
\[
\int_1^x f(t) ds(t) = \sum_{1 \leq n \leq x} f(n) = 
\sum_{1 \leq n \leq x} \frac{\log n}{n}.
\]

 Integrating by parts,
\begin{align*}
\int_1^x f(t) ds(t)&=s(x)f(x)-s(1)f(1) - \int_1^x s(t) df(t)\\
&=[x] \frac{\log x}{x} - \int_1^x [t] f'(t) dt\\
&=(x-\{x\}) \frac{\log x}{x} - \int_1^x(t-\{t\}) \frac{1-\log t}{t^2} dt\\
&=(x-\{x\})\frac{\log x}{x} -\int_1^x \frac{1-\log t}{t} dt
+ \int_1^x \{t\} \frac{1-\log t}{t^2} dt\\
&=(x-\{x\})\frac{\log x}{x} - \left(\log x - \frac{1}{2} (\log x)^2 \right)+\int_1^x \{t\} \frac{1-\log t}{t^2} dt.
\end{align*}
But
\[
\int_1^x \{t\} \frac{1-\log t}{t^2} dt=\int_1^\infty \{t\} \frac{1-\log t}{t^2} dt - 
\int_x^\infty \{t\} \frac{1-\log t}{t^2} dt.
\]
On the one hand,
\[
\left|\int_1^\infty \{t\} \frac{1-\log t}{t^2} dt \right| < \infty,
\]
and on the other hand,
\[
\left| \int_x^\infty \{t\} \frac{1-\log t}{t^2} dt \right|
\leq \left| \int_x^\infty \frac{1-\log t}{t^2} dt \right|
=\left| -\frac{\log x}{x} \right|.
\]
Therefore, writing $C=\int_1^\infty \{t\} \frac{1-\log t}{t^2} dt$, we have
\begin{align*}
\int_1^x f(t) ds(t) &= (x-\{x\})\frac{\log x}{x} - \left(\log x - \frac{1}{2} (\log x)^2 \right)
+C + O\left(\frac{\log x}{x}\right)\\
&=-\{x\} \frac{\log x}{x} + \frac{1}{2}(\log x)^2 + C  +O\left(\frac{\log x}{x}\right)\\
&=\frac{1}{2}(\log x)^2 + C  +O\left(\frac{\log x}{x}\right).
\end{align*}
Summarizing, as $x \to \infty$,
\[
\sum_{1 \leq n \leq x} \frac{\log n}{n} = \frac{1}{2}(\log x)^2 + C  +O\left(\frac{\log x}{x}\right).
\]